code/experimental/curve25519/Hacl.Impl.Curve25519.Lemmas.fsti
@@ -8,7 +8,3 @@ open Lib.ByteSequence
 val lemma_nat_from_uints64_le_4: b:lseq uint64 4 -> Lemma
   (nat_from_intseq_le b == v b.[0] + v b.[1] * pow2 64 +
     v b.[2] * pow2 64 * pow2 64 + v b.[3] * pow2 64 * pow2 64 * pow2 64)
-
-val lemma_uints64_from_bytes_le_nat:
-  #len:size_nat{8 * len <= max_size_t} -> b:lseq uint8 (8 * len) -> Lemma
-  (ensures  nat_from_intseq_le (uints_from_bytes_le #U64 #SEC #len b) == nat_from_bytes_le b)
